Checkpoint.

MQuinnEquiv.v
@@ -529,3 +529,59 @@ Example fold_bexp_ex2 :
                (AMinus (ANum 2) (APlus (ANum 1) (ANum 1)))))
     = BAnd (BEq (AId X) (AId Y)) BTrue.
 Proof. reflexivity. Qed.
+
+Fixpoint fold_constants_com (c : com) : com :=
+  match c with
+  | SKIP => SKIP
+  | i ::= a => CAss i (fold_constants_aexp a)
+  | c1 ;; c2 =>
+      (fold_constants_com c1) ;; (fold_constants_com c2)
+  | IFB b THEN c1 ELSE c2 FI =>
+      match fold_constants_bexp b with
+      | BTrue => fold_constants_com c1
+      | BFalse => fold_constants_com c2
+      | b1' => IFB b1' THEN (fold_constants_com c1)
+               ELSE (fold_constants_com c2) FI
+      end
+  | WHILE b DO c END =>
+      match fold_constants_bexp b with
+      | BTrue => WHILE BTrue DO SKIP END
+      | BFalse => SKIP
+      | b' => WHILE b' DO (fold_constants_com c) END
+      end
+  end.
+
+Example fold_com_ex1 :
+  fold_constants_com
+    (* Original program: *)
+    (X ::= APlus (ANum 4) (ANum 5);;
+     Y ::= AMinus (AId X) (ANum 3);;
+     IFB BEq (AMinus (AId X) (AId Y))
+             (APlus (ANum 2) (ANum 4)) THEN
+       SKIP
+     ELSE
+       Y ::= ANum 0
+     FI;;
+     IFB BLe (ANum 0)
+             (AMinus (ANum 4) (APlus (ANum 2) (ANum 1)))
+     THEN
+       Y ::= ANum 0
+     ELSE
+       SKIP
+     FI;;
+     WHILE BEq (AId Y) (ANum 0) DO
+       X ::= APlus (AId X) (ANum 1)
+     END)
+  = (* After constant folding: *)
+    (X ::= ANum 9;;
+     Y ::= AMinus (AId X) (ANum 3);;
+     IFB BEq (AMinus (AId X) (AId Y)) (ANum 6) THEN
+       SKIP
+     ELSE
+       (Y ::= ANum 0)
+     FI;;
+     Y ::= ANum 0;;
+     WHILE BEq (AId Y) (ANum 0) DO
+       X ::= APlus (AId X) (ANum 1)
+     END).
+Proof. reflexivity. Qed.
